theories/Math/DomainTheory.v
@@ -514,6 +514,48 @@ Proof with eauto.
   eapply G_compositionality... all: rewrite <- paco_eq_G...
 Qed.
 
+Theorem paco_yoneda (F : D -> D) (x : D) (y : D)
+  : x =< paco F y <-> (forall r : D, y =< r -> x =< paco F r).
+Proof.
+  split.
+  - intros x_le_paco_y r y_le_r. transitivity (paco F y); [exact x_le_paco_y | ].
+    revert r y_le_r. cofix CIH. intros r y_le_r z z_in.
+    apply unfold_paco in z_in. apply inv_paco' in z_in.
+    destruct z_in as [W [W_le z_in_FW]]. econs.
+    eapply mk_paco' with (WITNESS := W); auto.
+    intros a a_in_W. pose proof (W_le a a_in_W) as [a_in_y | a_in_paco_y].
+    + left. exact (y_le_r a a_in_y).
+    + right. exact (CIH r y_le_r a a_in_paco_y).
+  - ss!.
+Qed.
+
+Corollary pcofix1 (F : D -> D) (x : D) (y : D)
+  (COFIX1 : forall r : D, y =< r -> x =< r -> x =< paco F r)
+  : forall r : D, y =< r -> x =< paco F r.
+Proof.
+  eapply paco_yoneda.
+  set (Z := join_lattice x (paco F (join_lattice y x))).
+  enough (CLAIM : Z =< paco F y).
+  { intros z z_in_x. apply CLAIM. left. exact z_in_x. }
+  cofix CIH. intros z z_in_Z.
+  assert (z_in_paco_yx : z \in paco F (join_lattice y x)).
+  { destruct z_in_Z as [z_in_x | z_in_paco].
+    - eapply COFIX1.
+      + eapply le_join_lattice_introl. reflexivity.
+      + eapply le_join_lattice_intror. reflexivity.
+      + eapply z_in_x.
+    - exact z_in_paco.
+  }
+  apply unfold_paco in z_in_paco_yx. apply inv_paco' in z_in_paco_yx.
+  destruct z_in_paco_yx as [W [W_le z_in_FW]]. econs.
+  eapply mk_paco' with (WITNESS := W); auto.
+  intros a a_in_W. pose proof (W_le a a_in_W) as [a_in_yx | a_in_paco].
+  - destruct a_in_yx as [a_in_y | a_in_x].
+    + left. exact a_in_y.
+    + right. eapply CIH. left. exact a_in_x.
+  - right. eapply CIH. right. exact a_in_paco.
+Qed.
+
 End PACO.
 
 End COLA_THEORY.
